Redesign prophets.

theories/lang/typed_prophet.v
@@ -4,81 +4,296 @@ From caml5.lang Require Import
   notations
   proofmode.
 
-Record typed_prophet := {
-  typed_prophet_type : Type ;
-  typed_prophet_of_val : val → val → option typed_prophet_type ;
-  typed_prophet_to_val : typed_prophet_type → val * val ;
+Record typed_strong_prophet_spec := {
+  typed_strong_prophet_spec_type : Type ;
+  typed_strong_prophet_spec_of_val : val → val → option typed_strong_prophet_spec_type ;
+  typed_strong_prophet_spec_to_val : typed_strong_prophet_spec_type → val * val ;
 
-  typed_prophet_of_to_val proph w v :
-    (w, v) = typed_prophet_to_val proph →
-    typed_prophet_of_val w v = Some proph ;
+  typed_strong_prophet_spec_of_to_val proph w v :
+    (w, v) = typed_strong_prophet_spec_to_val proph →
+    typed_strong_prophet_spec_of_val w v = Some proph ;
 }.
-#[global] Arguments Build_typed_prophet {_ _ _} _.
+#[global] Arguments Build_typed_strong_prophet_spec {_ _ _} _ : assert.
 
-Section typed_prophet.
-  Context `{!heapGS Σ} (prophet : typed_prophet).
+Record typed_strong_prophet `{!heapGS Σ} := {
+  typed_strong_prophet_type : Type ;
+  typed_strong_prophet_to_val : typed_strong_prophet_type → val * val ;
 
-  #[local] Fixpoint typed_prophet_process prophs :=
+  typed_strong_prophet_model : proph_id → list typed_strong_prophet_type → iProp Σ ;
+
+  typed_strong_prophet_model_timeless p prophs :
+    Timeless (typed_strong_prophet_model p prophs) ;
+
+  typed_strong_prophet_model_exclusive p prophs1 prophs2 :
+    typed_strong_prophet_model p prophs1 -∗
+    typed_strong_prophet_model p prophs2 -∗
+    False ;
+
+  typed_strong_prophet_wp_new_proph E :
+    {{{ True }}}
+      NewProph @ E
+    {{{ p prophs, RET #p; typed_strong_prophet_model p prophs }}} ;
+
+  typed_strong_prophet_wp_resolve e v E p prophs Φ :
+    Atomic StronglyAtomic e →
+    to_val e = None →
+    typed_strong_prophet_model p prophs -∗
+    WP e @ E {{ w,
+      ∃ proph,
+      ⌜(w, v) = typed_strong_prophet_to_val proph⌝ ∗
+        ∀ prophs',
+        ⌜prophs = proph :: prophs'⌝ -∗
+        typed_strong_prophet_model p prophs' -∗
+        Φ w
+    }} -∗
+    WP Resolve e #p v @ E {{ Φ }} ;
+}.
+#[global] Arguments typed_strong_prophet _ {_} : assert.
+#[global] Arguments Build_typed_strong_prophet {_ _ _ _ _ _} _ _ _ : assert.
+#[global] Existing Instance typed_strong_prophet_model_timeless.
+#[global] Opaque typed_strong_prophet_model.
+
+Section make_typed_strong_prophet.
+  Context `{!heapGS Σ} (spec : typed_strong_prophet_spec).
+
+  #[local] Fixpoint make_typed_strong_prophet_process prophs :=
     match prophs with
     | [] =>
         []
     | (w, v) :: prophs =>
-        match prophet.(typed_prophet_of_val) w v with
+        match spec.(typed_strong_prophet_spec_of_val) w v with
         | None =>
             []
         | Some proph =>
-            proph :: typed_prophet_process prophs
+            proph :: make_typed_strong_prophet_process prophs
         end
     end.
-  Definition typed_prophet_model p prophs : iProp Σ :=
-    ∃ pvs,
-    ⌜prophs = typed_prophet_process pvs⌝ ∗ proph p pvs.
 
-  #[global] Instance typed_prophet_model_timeless p prophs :
-    Timeless (typed_prophet_model p prophs).
-  Proof.
-    apply _.
-  Qed.
+  Program Definition make_typed_strong_prophet := {|
+    typed_strong_prophet_type :=
+      spec.(typed_strong_prophet_spec_type) ;
+    typed_strong_prophet_to_val :=
+      spec.(typed_strong_prophet_spec_to_val) ;
 
-  Lemma typed_prophet_model_exclusive p prophs1 prophs2 :
-    typed_prophet_model p prophs1 -∗
-    typed_prophet_model p prophs2 -∗
-    False.
-  Proof.
+    typed_strong_prophet_model p prophs := (
+      ∃ pvs,
+      ⌜prophs = make_typed_strong_prophet_process pvs⌝ ∗
+      proph p pvs
+    )%I ;
+  |}.
+  Next Obligation.
     iIntros "* (%pvs1 & _ & Hp1) (%pvs2 & _ & Hp2)".
     iApply (proph_exclusive with "Hp1 Hp2").
   Qed.
-
-  Lemma typed_prophet_new_proph_spec E :
-    {{{ True }}}
-      NewProph @ E
-    {{{ p prophs, RET #p; typed_prophet_model p prophs }}}.
-  Proof.
-    iIntros "%Φ _ HΦ".
+  Next Obligation.
+    iIntros "* _ HΦ".
     wp_apply (wp_new_proph with "[//]"). iIntros "%pvs %p Hp".
     iApply "HΦ". iExists pvs. auto with iFrame.
   Qed.
-
-  Lemma typed_prophet_resolve_spec e v E p prophs Φ :
-    Atomic StronglyAtomic e →
-    to_val e = None →
-    typed_prophet_model p prophs -∗
-    WP e @ E {{ w,
-      ∃ proph,
-      ⌜(w, v) = prophet.(typed_prophet_to_val) proph⌝ ∗
-        ∀ prophs',
-        ⌜prophs = proph :: prophs'⌝ -∗
-        typed_prophet_model p prophs' -∗
-        Φ w
-    }} -∗
-    WP Resolve e #p v @ E {{ Φ }}.
-  Proof.
-    iIntros "% % (%pvs & %Hprophs & Hp) HΦ".
+  Next Obligation.
+    iIntros "* % % (%pvs & %Hprophs & Hp) HΦ".
     wp_apply (wp_resolve with "Hp"); first done.
     wp_apply (wp_wand with "HΦ"). iIntros "%w (%proph & % & HΦ) %pvs' -> Hp".
-    rewrite /= (typed_prophet_of_to_val _ proph) in Hprophs; last done.
+    rewrite /= (typed_strong_prophet_spec_of_to_val _ proph) in Hprophs; last done.
     iApply "HΦ"; first done. iExists pvs'. auto with iFrame.
   Qed.
-End typed_prophet.
+End make_typed_strong_prophet.
 
+Record typed_prophet_spec := {
+  typed_prophet_spec_type : Type ;
+  typed_prophet_spec_of_val : val → option typed_prophet_spec_type ;
+  typed_prophet_spec_to_val : typed_prophet_spec_type → val ;
+
+  typed_prophet_spec_of_to_val proph v :
+    v = typed_prophet_spec_to_val proph →
+    typed_prophet_spec_of_val v = Some proph ;
+}.
+#[global] Arguments Build_typed_prophet_spec {_ _ _} _ : assert.
+
+Record typed_prophet `{!heapGS Σ} := {
+  typed_prophet_type : Type ;
+  typed_prophet_to_val : typed_prophet_type → val ;
+
+  typed_prophet_model : proph_id → list typed_prophet_type → iProp Σ ;
+
+  typed_prophet_model_timeless p prophs :
+    Timeless (typed_prophet_model p prophs) ;
+
+  typed_prophet_model_exclusive p prophs1 prophs2 :
+    typed_prophet_model p prophs1 -∗
+    typed_prophet_model p prophs2 -∗
+    False ;
+
+  typed_prophet_wp_new_proph E :
+    {{{ True }}}
+      NewProph @ E
+    {{{ p prophs, RET #p; typed_prophet_model p prophs }}} ;
+
+  typed_prophet_wp_resolve proph e v E p prophs Φ :
+    Atomic StronglyAtomic e →
+    to_val e = None →
+    v = typed_prophet_to_val proph →
+    typed_prophet_model p prophs -∗
+    WP e @ E {{ w,
+      ∀ prophs',
+      ⌜prophs = proph :: prophs'⌝ -∗
+      typed_prophet_model p prophs' -∗
+      Φ w
+    }} -∗
+    WP Resolve e #p v @ E {{ Φ }} ;
+}.
+#[global] Arguments typed_prophet _ {_} : assert.
+#[global] Arguments Build_typed_prophet {_ _ _ _ _ _} _ _ _ : assert.
+#[global] Existing Instance typed_prophet_model_timeless.
 #[global] Opaque typed_prophet_model.
+
+Section make_typed_prophet.
+  Context `{!heapGS Σ} (spec : typed_prophet_spec).
+
+  #[local] Program Definition make_typed_prophet_strong_prophet_spec := {|
+    typed_strong_prophet_spec_type :=
+      val * spec.(typed_prophet_spec_type) ;
+    typed_strong_prophet_spec_of_val w v :=
+      match spec.(typed_prophet_spec_of_val) v with
+      | None => None
+      | Some proph => Some (w, proph)
+      end ;
+    typed_strong_prophet_spec_to_val '(w, proph) :=
+      (w, spec.(typed_prophet_spec_to_val) proph) ;
+  |}.
+  Next Obligation.
+    intros (w & proph) _w v [= -> ->].
+    erewrite spec.(typed_prophet_spec_of_to_val); done.
+  Qed.
+
+  #[local] Definition make_typed_prophet_strong_prophet :=
+    make_typed_strong_prophet make_typed_prophet_strong_prophet_spec.
+
+  Program Definition make_typed_prophet := {|
+    typed_prophet_type :=
+      spec.(typed_prophet_spec_type) ;
+    typed_prophet_to_val :=
+      spec.(typed_prophet_spec_to_val) ;
+
+    typed_prophet_model p prophs := (
+      ∃ sprophs,
+      ⌜prophs = sprophs.*2⌝ ∗
+      make_typed_prophet_strong_prophet.(typed_strong_prophet_model) p sprophs
+    )%I ;
+  |}.
+  Next Obligation.
+    iIntros "* (%sprophs1 & _ & Hmodel1) (%sprophs2 & _ & Hmodel2)".
+    iApply (typed_strong_prophet_model_exclusive with "Hmodel1 Hmodel2").
+  Qed.
+  Next Obligation.
+    iIntros "* _ HΦ".
+    wp_apply (make_typed_prophet_strong_prophet.(typed_strong_prophet_wp_new_proph) with "[//]"). iIntros "%p %sprophs Hmodel".
+    iApply "HΦ". iExists sprophs. auto with iFrame.
+  Qed.
+  Next Obligation.
+    iIntros "*" (? ? ->) "(%sprophs & -> & Hmodel) HΦ".
+    wp_apply (typed_strong_prophet_wp_resolve with "Hmodel"); first done.
+    wp_apply (wp_wand with "HΦ"). iIntros "%w HΦ".
+    iExists (w, proph). iSplit; first done. iIntros "%sprophs' -> Hmodel".
+    iApply ("HΦ" with "[//]"). iExists sprophs'. auto with iFrame.
+  Qed.
+End make_typed_prophet.
+
+Record typed_prophet1_spec := {
+  typed_prophet1_spec_type : Type ;
+  typed_prophet1_spec_of_val : val → option typed_prophet1_spec_type ;
+  typed_prophet1_spec_to_val : typed_prophet1_spec_type → val ;
+
+  typed_prophet1_spec_type_inhabited :
+    Inhabited typed_prophet1_spec_type ;
+
+  typed_prophet1_spec_of_to_val proph v :
+    v = typed_prophet1_spec_to_val proph →
+    typed_prophet1_spec_of_val v = Some proph ;
+}.
+#[global] Arguments Build_typed_prophet1_spec {_ _ _ _} _ : assert.
+#[global] Existing Instance typed_prophet1_spec_type_inhabited.
+
+Program Coercion typed_prophet1_spec_of_prophet_spec spec := {|
+  typed_prophet_spec_type :=
+    spec.(typed_prophet1_spec_type) ;
+  typed_prophet_spec_of_val :=
+    spec.(typed_prophet1_spec_of_val) ;
+  typed_prophet_spec_to_val :=
+    spec.(typed_prophet1_spec_to_val) ;
+|}.
+Next Obligation.
+  apply typed_prophet1_spec_of_to_val.
+Qed.
+
+Record typed_prophet1 `{!heapGS Σ} := {
+  typed_prophet1_type : Type ;
+  typed_prophet1_to_val : typed_prophet1_type → val ;
+
+  typed_prophet1_model : proph_id → typed_prophet1_type → iProp Σ ;
+
+  typed_prophet1_model_timeless p proph :
+    Timeless (typed_prophet1_model p proph) ;
+
+  typed_prophet1_model_exclusive p proph1 proph2 :
+    typed_prophet1_model p proph1 -∗
+    typed_prophet1_model p proph2 -∗
+    False ;
+
+  typed_prophet1_wp_new_proph E :
+    {{{ True }}}
+      NewProph @ E
+    {{{ p proph, RET #p; typed_prophet1_model p proph }}} ;
+
+  typed_prophet1_wp_resolve proph e v E p proph' Φ :
+    Atomic StronglyAtomic e →
+    to_val e = None →
+    v = typed_prophet1_to_val proph →
+    typed_prophet1_model p proph' -∗
+    WP e @ E {{ w, ⌜proph' = proph⌝ -∗ Φ w }} -∗
+    WP Resolve e #p v @ E {{ Φ }} ;
+}.
+#[global] Arguments typed_prophet1 _ {_} : assert.
+#[global] Arguments Build_typed_prophet1 {_ _ _ _ _ _} _ _ _ : assert.
+#[global] Existing Instance typed_prophet1_model_timeless.
+#[global] Opaque typed_prophet1_model.
+
+Section make_typed_prophet1.
+  Context `{!heapGS Σ} (spec : typed_prophet1_spec).
+
+  #[local] Definition make_typed_prophet1_prophet :=
+    make_typed_prophet spec.
+
+  Program Definition make_typed_prophet1 := {|
+    typed_prophet1_type :=
+      spec.(typed_prophet_spec_type) ;
+    typed_prophet1_to_val :=
+      spec.(typed_prophet_spec_to_val) ;
+
+    typed_prophet1_model p proph := (
+      ∃ prophs,
+      make_typed_prophet1_prophet.(typed_prophet_model) p prophs ∗
+      ⌜if prophs is proph' :: _ then proph' = proph else True⌝
+    )%I ;
+  |}.
+  Next Obligation.
+    done.
+  Qed.
+  Next Obligation.
+    iIntros "* (%prophs1 & Hmodel1 & _) (%prophs2 & Hmodel2 & _)".
+    iApply (typed_prophet_model_exclusive with "Hmodel1 Hmodel2").
+  Qed.
+  Next Obligation.
+    iIntros "* _ HΦ".
+    wp_apply (make_typed_prophet1_prophet.(typed_prophet_wp_new_proph) with "[//]"). iIntros "%p %prophs Hmodel".
+    destruct prophs as [| proph prophs'] eqn:Heq;
+      [iApply ("HΦ" $! p inhabitant) | iApply ("HΦ" $! p proph)];
+      iExists prophs; rewrite Heq; iFrame; done.
+  Qed.
+  Next Obligation.
+    iIntros "*" (? ? ->) "(%prophs & Hmodel & %) HΦ".
+    wp_apply (typed_prophet_wp_resolve with "Hmodel"); [done.. |].
+    iApply (wp_wand with "HΦ"). iIntros "%v HΦ %prophs' -> _".
+    iApply "HΦ". done.
+  Qed.
+End make_typed_prophet1.
